theories/type_systems/stlc/lang.v
@@ -35,10 +35,6 @@ Fixpoint subst (x : string) (es : expr) (e : expr)  : expr :=
   | Plus e1 e2 => Plus (subst x es e1) (subst x es e2)
   end.
 
-(** ** §1.1: Operational Semantics *)
-
-(** *** Small-Step Structural Semantics *)
-
 (** A predicate which holds true whenever an
 expression is a value. *)
 Definition is_val (e : expr) : Prop :=
@@ -47,6 +43,10 @@ Definition is_val (e : expr) : Prop :=
   | Lam x e => True
   | _ => False
   end.
+
+(** ** §1.1: Operational Semantics *)
+
+(** *** Small-Step Structural Semantics *)
 
 (* We use right-to-left evaluation order,
    which means in a binary term (e.g., e1 + e2),
@@ -160,9 +160,10 @@ End examples.
 
 (** *** Big-Step Semantics *)
 
-(** To formalize big-step semantics, we have to define not just a predicate [is_val]
-but an actual *type* of values, [val]. We also define functions to convert between
-expressions and values and show their basic properties. *)
+(** To formalize big-step semantics, we have to define not just a predicate
+[is_val] but an actual Coq *type* of values, [val]. We also define functions to
+convert between expressions and values and show their basic properties, and
+their relationship with [is_val]. *)
 
 Inductive val :=
   | LitIntV (n: Z)
@@ -194,36 +195,28 @@ Proof.
   all: injection 1 as <-; simpl; reflexivity.
 Qed.
 
-Lemma is_val_spec e : is_val e <-> exists v, to_val e = Some v.
+(** We can rewrite terms that are values into the form [of_val v]. *)
+Lemma is_val_make_val e : is_val e -> exists v, e = of_val v.
 Proof.
-  destruct e; simpl.
-  (* With [all:], we can apply a tactic to all open subgoals. *)
-  all: split; [intros H|intros [v H]]; try done.
-  (* [done] can solve almost all of these goals, but it cannot show these two
-  existential quantifiers. We could prove them individually by hand now, but
-  then we have to manually state the witness that proves the existential.
-  Instead we can have Coq infer the witness by using evars (existential
-  variables) that we have already seen before with [eapply]: The [eexists]
-  tactic turns the quantified variable into an evar. *)
-  all: eexists.
-  (* Now both of these goals can be proven by reflexivity, which implicitly
-  makes Coq choose the right witness for the existentials. *)
-  all: done.
+  intros He.
+  (* [cut] is "it suffices to show". *)
+  cut (exists v, to_val e = Some v).
+  { intros [v ?]. exists v. symmetry. apply of_to_val. done. }
+  (* Handle the rest. Many cases are simple contradictions. *)
+  destruct e; simpl; try contradiction.
+  (* We could prove the remaining goals individually by hand now, but then we
+  have to manually state the witness that proves the existential. Instead we can
+  have Coq infer the witness by using evars (existential variables) that we have
+  already seen before with [eapply]: The [eexists] tactic turns the quantified
+  variable into an evar. *)
+  all: eexists; done.
 Qed.
 
-(* This is the most useful lemma: when we know something is a value,
-we can rewrite it into the form [of_val v] for some [v]. This will
-then let us use other lemmas that require [of_val]. *)
-Lemma is_val_rewrite e :
-  is_val e -> exists v, e = of_val v.
+(** In fact, [is_val] is fully characterized by these new operations. *)
+Lemma is_val_spec e : is_val e <-> exists v, e = of_val v.
 Proof.
-  intros [v Hv]%is_val_spec. exists v.
-  apply of_to_val in Hv. done.
-Qed.
-
-Lemma is_val_of_val v : is_val (of_val v).
-Proof.
-  apply is_val_spec. rewrite to_of_val. by eexists.
+  split; first by apply is_val_make_val.
+  intros [v ->]. destruct v; done.
 Qed.
 
 (** Now we are finally ready to define the actual big-step evaluation relation. *)
@@ -315,8 +308,13 @@ Proof.
   induction 1; eauto.
 Qed.
 
-(** For this proof we tell [eauto] about another lemma that we will need.
-[Hint Resolve] adds an individual lemma to the hint database. *)
+(** For this proof we tell [eauto] about another lemma that we will need:
+showing that [of_val v] is always a value. *)
+Lemma is_val_of_val v : is_val (of_val v).
+Proof.
+  apply is_val_spec. eexists. done.
+Qed.
+(* [Hint Resolve] adds an individual lemma to the hint database. *)
 #[export] Hint Resolve is_val_of_val : core.
 
 Lemma big_step_step e v :
@@ -337,7 +335,8 @@ Qed.
 (** The opposite direction will be an exercise. *)
 
 (** *** Contextual Semantics *)
-(** Base reduction *)
+
+(** * Base reduction *)
 Inductive base_step : expr -> expr -> Prop :=
   | BetaS x e1 e2 e' :
      is_val e2 ->
@@ -348,6 +347,8 @@ Inductive base_step : expr -> expr -> Prop :=
      e2 = (LitInt n2) ->
      (n1 + n2)%Z = n3 ->
      base_step (Plus e1 e2) (LitInt n3).
+
+(** * Evaluation contexts *)
 
 (** On paper, we defined evaluation contexts roughly like this. *)
 Module ectx_on_paper.
@@ -420,13 +421,6 @@ Proof. reflexivity. Qed.
 
 End ectx_on_paper_comparison.
 
-Inductive contextual_step (e1 : expr) (e2 : expr) : Prop :=
-  EctxStep K e1' e2' :
-    e1 = fill K e1' ->
-    e2 = fill K e2' ->
-    base_step e1' e2' ->
-    contextual_step e1 e2.
-
 (** Composition of contexts.
 This is where using a list starts paying off.
 Remember that the innermost items [Ki] go first. *)
@@ -450,6 +444,15 @@ definitional equalities can be very useful, and that's why we prefer
 Definition empty_ectx : ectx := [].
 Lemma fill_empty e : fill empty_ectx e = e.
 Proof. done. Qed.
+
+(** * Contextual step relation *)
+
+Inductive contextual_step (e1 : expr) (e2 : expr) : Prop :=
+  EctxStep K e1' e2' :
+    e1 = fill K e1' ->
+    e2 = fill K e2' ->
+    base_step e1' e2' ->
+    contextual_step e1 e2.
 
 (** Basic lemmas about the contextual semantics *)
 
