theories/type_systems/stlc_de_bruijn/bigstep.v
@@ -1,0 +1,34 @@
+From ffpl.lib Require Import prelude.
+From ffpl.type_systems.stlc_de_bruijn Require Import lang.
+
+(** *** Big-Step Semantics *)
+
+Inductive big_step : expr -> val -> Prop :=
+  | BsLitInt (n : Z) :
+      big_step (LitInt n) (LitIntV n)
+  | BsLam (e : expr) :
+      big_step (Lam e) (LamV e)
+  | BsPlus e1 e2 (z1 z2 : Z) :
+      big_step e1 (LitIntV z1) ->
+      big_step e2 (LitIntV z2) ->
+      big_step (Plus e1 e2) (LitIntV (z1 + z2))%Z
+  | BisApp e1 e2 e v2 v :
+      big_step e1 (LamV e) ->
+      big_step e2 v2 ->
+      big_step e.[of_val v2/] v ->
+      big_step (App e1 e2) v.
+#[export] Hint Constructors big_step : core.
+
+(** We can show that values behave the way they should. *)
+Lemma big_step_vals (v : val) : big_step (of_val v) v.
+Proof.
+  induction v; try constructor; done.
+Qed.
+
+Lemma big_step_inv_vals (v w : val) : big_step (of_val v) w -> v = w.
+Proof.
+  (** [inversion 1] means "do inversion on the first assumption in the goal",
+  i.e., it is the same as [intros H; inversion H]. *)
+  revert w.
+  induction v; inversion 1; try reflexivity.
+Qed.
