theories/type_systems/stlc_de_bruijn/logrel.v
@@ -1,0 +1,226 @@
+From stdpp Require Import base relations.
+From ffpl.lib Require Import prelude sets maps.
+From ffpl.type_systems.stlc_de_bruijn Require Import lang notation bigstep types.
+From Equations Require Import Equations.
+
+(** The next command makes Coq guess the type of a variable based on its name.
+*)
+Implicit Types
+  (Gamma : typing_context)
+  (v : val)
+  (e : expr)
+  (A : type).
+
+
+(** ** Definition of the logical relation. *)
+
+(** The logical relation is defined mutually recursively on expressions and values.
+To encode this in Coq, we define a type that is "expression or value", and then
+define the relation on that. The [inj_val] and [inj_expr] constructors
+are used to convert values/expressions into that shared type. *)
+Inductive val_or_expr : Type :=
+| inj_val : val -> val_or_expr
+| inj_expr : expr -> val_or_expr.
+
+(**
+  In Coq, we need to make argument why the logical relation is well-defined precise:
+  This holds true in particular for the mutual recursion between the value relation and the expression relation
+   (note that the value relation is defined in terms of the expression relation, and vice versa).
+  We therefore define a termination measure [mut_measure] that makes sure that for each recursive call, we either
+   - decrease the size of the type
+   - or switch from the expression case to the value case.
+
+  We use the Equations package to define the logical relation, as it's tedious to make the termination
+   argument work with Coq's built-in support for recursive functions---but under the hood, Equations also
+   just encodes it as a Coq Fixpoint.
+ *)
+
+(* The [type_size] function just structurally descends, essentially taking the size of the "type tree". *)
+Equations type_size (t : type) : nat :=
+  type_size Int := 1;
+  type_size (Fun A B) := type_size A + type_size B + 1.
+
+(* The definition of the expression relation uses the value relation -- therefore, it needs to be larger, and we add [1]. *)
+Equations mut_measure (ve : val_or_expr) (t : type) : nat :=
+  mut_measure (inj_expr e) t := 1 + type_size t;
+  mut_measure (inj_val v) t := type_size t.
+
+
+(** The main definition of the logical relation.
+
+  The [by wf ..] part tells Equations to use [mut_measure] for the well-formedness argument.
+  It turns out that we get nicer simplification behavior for the expression case
+  by putting the [val + expr] argument first.
+ *)
+Equations type_interp (ve : val_or_expr) (t : type) : Prop by wf (mut_measure ve t) := {
+  type_interp (inj_val v) Int =>
+    exists z : Z, v = z ;
+  type_interp (inj_val v) (A -> B) =>
+    exists e, v = LamV e /\
+      forall v',
+        type_interp (inj_val v') A ->
+        type_interp (inj_expr e.[of_val v'/]) B;
+
+  type_interp (inj_expr e) t =>
+    exists v, big_step e v /\ type_interp (inj_val v) t
+}.
+Next Obligation.
+  (** [simp] is a tactic provided by [Equations]. It rewrites with the defining equations of the definition.
+    [simpl]/[cbn] will NOT unfold definitions made with Equations.
+   *)
+  repeat simp mut_measure; simp type_size; lia.
+Qed.
+Next Obligation.
+  simp mut_measure. simp type_size.
+  destruct A; repeat simp mut_measure; repeat simp type_size; lia.
+Qed.
+
+(** We derive the expression/value relation.
+Note that these are [Notation], not [Definition]: we are not introducing new
+terms here that have to be unfolded, we are merly introducing a notational short-hand.
+This means tactics like [simp] can still "see" the underlying [type_interp],
+which makes proof a lot more pleasant. *)
+Notation sem_val_rel t v := (type_interp (inj_val v) t).
+Notation sem_expr_rel t e := (type_interp (inj_expr e) t).
+
+(** *** Semantic typing of contexts *)
+
+(** As before, we use maps to [expr] rather than [val] to represent "value
+substitutions", this time because they can be directly used as substitutions with
+Autosubst. *)
+Implicit Types (gamma : var -> expr).
+
+Definition sem_ctx_rel Gamma gamma :=
+  forall x A, Gamma !! x = Some A -> exists v, gamma x = of_val v /\ sem_val_rel A v.
+
+(** The semantic typing judgment *)
+Definition sem_typed Gamma e A :=
+  forall gamma, sem_ctx_rel Gamma gamma -> sem_expr_rel A e.[gamma].
+Notation "Gamma |= e : A" := (sem_typed Gamma e A) (at level 74, e, A at next level).
+
+(** We start by proving a couple of helper lemmas that will be useful later. *)
+
+Lemma sem_ctx_rel_nil gamma : sem_ctx_rel [] gamma.
+Proof.
+  intros x A. rewrite lookup_nil. done.
+Qed.
+
+Lemma sem_ctx_rel_cons Gamma gamma v A :
+  sem_val_rel A v ->
+  sem_ctx_rel Gamma gamma ->
+  sem_ctx_rel (A :: Gamma) (of_val v .: gamma).
+Proof.
+  intros Hv Hgamma [|x] B; simpl.
+  - intros [= <-]. eauto.
+  - eapply Hgamma.
+Qed.
+
+(** Lemma 17: Value Inclusion *)
+Lemma val_inclusion A v :
+  sem_val_rel A v -> sem_expr_rel A (of_val v).
+Proof.
+  intros Hv. simp type_interp. exists v.
+  split; last done. apply big_step_vals.
+Qed.
+
+(** *** Compatibility lemmas *)
+
+(** Lemma 19 *)
+Lemma compat_int Gamma z : Gamma |= (LitInt z) : Int.
+Proof.
+  intros gamma _. simpl. apply (val_inclusion _ z).
+  simp type_interp. eauto.
+Qed.
+
+(** Lemma 20 *)
+Lemma compat_var Gamma x A :
+  Gamma !! x = Some A ->
+  Gamma |= (Var x) : A.
+Proof.
+  intros Hx gamma Hctx; simpl.
+  specialize (Hctx _ _ Hx) as (v & Hlookup & Hv).
+  rewrite Hlookup. apply val_inclusion. done.
+Qed.
+
+(** Lemma 21 *)
+Lemma compat_add Gamma e1 e2 :
+  Gamma |= e1 : Int ->
+  Gamma |= e2 : Int ->
+  Gamma |= (e1 + e2) : Int.
+Proof.
+  intros He1 He2 gamma Hctx. simpl.
+  simp type_interp.
+  specialize (He1 _ Hctx). specialize (He2 _ Hctx).
+  simp type_interp in He1. simp type_interp in He2.
+
+  destruct He1 as (v1 & Hb1 & Hv1).
+  destruct He2 as (v2 & Hb2 & Hv2).
+  simp type_interp in Hv1, Hv2.
+  destruct Hv1 as (z1 & ->). destruct Hv2 as (z2 & ->).
+
+  exists (z1 + z2)%Z. split.
+  - constructor; done.
+  - exists (z1 + z2)%Z. done.
+Qed.
+
+(** Lemma 22 *)
+Lemma compat_app Gamma e1 e2 A B :
+  Gamma |= e1 : (A -> B) ->
+  Gamma |= e2 : A ->
+  Gamma |= (e1 e2) : B.
+Proof.
+  intros Hfun Harg gamma Hctx; simpl.
+  specialize (Hfun _ Hctx). simp type_interp in Hfun. destruct Hfun as (v1 & Hbs1 & Hv1).
+  simp type_interp in Hv1. destruct Hv1 as (e & -> & Hv1).
+  specialize (Harg _ Hctx). simp type_interp in Harg.
+  destruct Harg as (v2 & Hbs2 & Hv2).
+
+  apply Hv1 in Hv2.
+  simp type_interp in Hv2. destruct Hv2 as (v & Hbsv & Hv).
+
+  simp type_interp.
+  exists v.
+  split; last done.
+  eauto.
+Qed.
+
+(** Lemma 23 *)
+Lemma compat_lam Gamma e A B :
+  (A :: Gamma) |= e : B ->
+  Gamma |= (Lam e) : (A -> B).
+Proof.
+  intros Hbody gamma Hctxt. asimpl.
+  apply (val_inclusion _ (lam: _)%V).
+  simp type_interp.
+  eexists _. split; first done.
+
+  intros v Hv.
+  asimpl. apply (Hbody (of_val v .: gamma)).
+  eapply sem_ctx_rel_cons; done.
+Qed.
+
+(** Theorem 24 *)
+Theorem sem_soundness Gamma e A :
+  (Gamma |- e : A)%ty ->
+  Gamma |= e : A.
+Proof.
+  induction 1.
+  - by apply compat_var.
+  - by apply compat_lam.
+  - by apply compat_int.
+  - by eapply compat_app.
+  - by apply compat_add.
+Qed.
+
+(** Corollary 25 *)
+Corollary termination e A :
+  ([] |- e : A)%ty ->
+  exists v, big_step e v.
+Proof.
+  intros Hsem%sem_soundness.
+  specialize (Hsem ids).
+  simp type_interp in Hsem.
+  destruct Hsem as (v & Hbs & _).
+  { eapply sem_ctx_rel_nil. }
+  asimpl in Hbs. eauto.
+Qed.
