theories/type_systems/stlc_de_bruijn/notation.v
@@ -1,5 +1,5 @@
 From ffpl.lib Require Import prelude.
-From ffpl.type_systems.stlc_extended Require Export lang.
+From ffpl.type_systems.stlc_de_bruijn Require Export lang.
 
 (* We declare two notation scopes, one for values and one for expressions.
    Afterwards, we add notations to them, which then do not interfere with
@@ -19,27 +19,22 @@ Coercion of_val : val >-> expr.
 Coercion LitInt : Z >-> expr.
 Coercion LitIntV : Z >-> val.
 Coercion App : expr >-> Funclass.
-Coercion Var : string >-> expr.
 
 (* In the expr and val scopes, we want numbers to be interpreted as integers. *)
 Number Notation Z Z.of_num_int Z.to_num_int : expr_scope.
 Number Notation Z Z.of_num_int Z.to_num_int : val_scope.
 
+(* Notation for de-Bruijn indices *)
+Notation "'^' n" := (Var n%nat)
+  (at level 8, format "'^' n") : expr_scope.
+
 (* Notation for particular expression.s *)
 Notation "e1 + e2" := (Plus e1%E e2%E) : expr_scope.
 
-(* The breaking point '/  ' makes sure that the body of the lam: is indented
-by two spaces in case the whole lam: does not fit on a single line. *)
-Notation "'lam:' x , e" := (Lam x e%E)
-  (at level 200, x at level 1, e at level 200,
-   format "'[' 'lam:'  x ,  '/  ' e ']'") : expr_scope.
-Notation "'lam:' x y .. z , e" := (Lam x (Lam y .. (Lam z e%E) ..))
-  (at level 200, x, y, z at level 1, e at level 200,
-   format "'[' 'lam:'  x  y  ..  z ,  '/  ' e ']'") : expr_scope.
+Notation "'lam:' e" := (Lam e%E)
+  (at level 200, e at level 200,
+   format "'[' 'lam:'  e ']'") : expr_scope.
 
-Notation "'lam:' x , e" := (LamV x e%E)
-  (at level 200, x at level 1, e at level 200,
-   format "'[' 'lam:'  x ,  '/  ' e ']'") : val_scope.
-Notation "'lam:' x y .. z , e" := (LamV x (Lam y .. (Lam z e%E) .. ))
-  (at level 200, x, y, z at level 1, e at level 200,
-   format "'[' 'lam:'  x  y  ..  z ,  '/  ' e ']'") : val_scope.
+Notation "'lam:' e" := (LamV e%E)
+  (at level 200, e at level 200,
+   format "'[' 'lam:'  e ']'") : val_scope.
