theories/type_systems/stlc_de_bruijn/subst.v
@@ -1,0 +1,94 @@
+From ffpl.lib Require Import prelude.
+From ffpl.type_systems.stlc_de_bruijn Require Import lang notation.
+
+(* Autosubst magically defined a substitution function for us.
+Let's explore it with some examples. *)
+Definition e1 : expr := ^0 + 1. (* x + 1 *)
+Compute e1.[LitInt 2/].
+
+Definition e2 : expr := lam: e1. (* lam: x, x + 1 *)
+Compute e2.[LitInt 2/].
+
+(* Things get intersting when we substitute under binders.
+Substituting closed terms works pretty directly. *)
+Definition e3 : expr := lam: ^1. (* lam: x, y. *)
+Compute e3.[LitInt 2/].
+Compute e3.[e2/].
+
+(* But when we substitute an open term... *)
+Compute e3.[e1/].
+(* ... the free variables need to be updated since they are now
+below more binders! The "^0" in [e1] changes to "^1" since it must
+now "skip over" the "lam:" in [e3]. *)
+
+(* When there are multiple free variables in a term, substituting one "shifts" the others down. *)
+Compute (^0 + ^1)%E.[LitInt 4/].
+(* Now that ^0 is gone, the former ^1 is the "first" variable. *)
+
+(* With de-Bruijn indices, we typically use "parallel substitution" as the primitive building block.
+We previously encountered parallel substitution when defining the logical relation.
+A parallel substitution [sigma] has type [var -> expr], and the operation [e.[sigma]]
+applies [sigma] everywhere in [e]. This is like our previous [subst_map], except that
+it is a *total* function: all variables must be mapped to some term.
+Variables that we want to leave unchanged can just map to themselves.
+
+To define substitution of the "first" variable (^0) with some term [e], we construct
+a suitable parallel substitution: *)
+Definition subst_from_single e : var -> expr := fun n =>
+  match n with
+  | O => e
+  (* Everything else gets decremented by one since the first variable is gone! *)
+  | S n => Var n
+  end.
+(* We can show that this is equivalent to what autosubst does. *)
+Lemma subst_from_single_correct e1 e2 :
+  e1.[subst_from_single e2] = e1.[e2/].
+Proof. reflexivity. Qed.
+
+(* Parallel substitution is defined by the following equations. *)
+Lemma subst_plus sigma (e1 e2 : expr) :
+  (e1 + e2)%E.[sigma] = (e1.[sigma] + e2.[sigma])%E.
+Proof. reflexivity. Qed.
+Lemma subst_int sigma (n : Z) :
+  (LitInt n).[sigma] = LitInt n.
+Proof. reflexivity. Qed.
+Lemma subst_app sigma (e1 e2 : expr) :
+  (e1 e2).[sigma] = e1.[sigma] e2.[sigma].
+Proof. reflexivity. Qed.
+Lemma subst_var sigma (x : var) :
+  (Var x).[sigma] = sigma x.
+Proof. reflexivity. Qed.
+(* So far this is just structural recursion over the term,
+looking up variables when we reach them. Things get interesting
+when we have to traverse below a binder: we need to "shift"
+the substitution by one. Inside this lambda, [0] needs to remain unchanged
+(since it refers to the binder we just went through), and everything else
+needs to account for the fact that it is now under one more lambda. *)
+Definition subst_up (sigma : var -> expr) : var -> expr := fun n =>
+  match n with
+  | O => Var O
+  | S n => (sigma n).[fun m => Var (S m)]
+  end.
+Lemma subst_lam sigma e :
+  (Lam e).[sigma] = Lam (e.[subst_up sigma]).
+Proof.
+  (* This time we need to unfold some autosubst internals to show that
+  this is really the same thing. *)
+  asimpl. f_equal. f_equal. f_ext. intros [|x]; simpl.
+  - reflexivity.
+  - asimpl. reflexivity.
+Qed.
+
+(* There is just one problem with this definition: it is recursive! In
+[subst_up], we used substitution, but we are currently trying to *define*
+substitution. Resolving this recursion involves introducing a notion of
+"renamings" of type [var -> var] and first defining how to substitute renamings
+before we can define how to apply full substitutions. [subst_up] can be defined
+using just renamins, and renamings can be defined without [subst_up] (they need
+a [ren_up], but that one can be defined directly without needing any kind of
+substitution). It's all a bit cumbersome, but lucky enough, we don't have to
+worry about this -- Autosubst does all that work for us.
+
+The upshot is that the definition given above *is* well-formed, it just takes a
+bit of work to convince Coq of that fact. Conveniently, we don't have to do that
+work. *)
