theories/type_systems/stlc_de_bruijn/types.v
@@ -1,0 +1,315 @@
+From stdpp Require Import base relations tactics.
+From ffpl.lib Require Import prelude sets maps.
+From ffpl.type_systems.stlc_de_bruijn Require Import lang notation.
+
+(** ** Syntactic typing *)
+(** In the Coq formalization, we exclusively define runtime typing (Curry-style). *)
+
+Inductive type : Set :=
+  | Int
+  | Fun (A B : type).
+
+(** Now that variables are using De Bruijn indices, typing contexts are just lists of types.
+On paper we write "Gamma, A" to extend a context, but lists in Coq are indexed
+from the left so this will correspond to [A :: Gamma]. *)
+Notation typing_context := (list type).
+
+Implicit Types
+  (Gamma : typing_context)
+  (v : val)
+  (e : expr)
+  (A : type).
+
+(** We define notation for types in a new scope with delimiter [ty].
+  See below for an example. *)
+Declare Scope FType_scope.
+Delimit Scope FType_scope with ty.
+Bind Scope FType_scope with type.
+Infix "->" := Fun : FType_scope.
+
+(** Typing rules *)
+(** We need to reserve the notation beforehand to already use it when defining the
+   typing rules. *)
+Reserved Notation "Gamma |- e : A" (at level 74, e, A at next level).
+Inductive syn_typed : typing_context -> expr -> type -> Prop :=
+  | type_var Gamma x A :
+      (* lookup the variable in the context *)
+      Gamma !! x = Some A ->
+      Gamma |- (Var x) : A
+  | type_lam Gamma e A B :
+      (* add a new type assignment to the context *)
+      (A :: Gamma) |- e : B ->
+      Gamma |- (Lam e) : (A -> B)
+  | type_int Gamma z :
+      Gamma |- (LitInt z) : Int
+  | type_app Gamma e1 e2 A B :
+      Gamma |- e1 : (A -> B) ->
+      Gamma |- e2 : A ->
+      Gamma |- e1 e2 : B
+  | type_add Gamma e1 e2 :
+      Gamma |- e1 : Int ->
+      Gamma |- e2 : Int ->
+      Gamma |- e1 + e2 : Int
+where "Gamma |- e : A" := (syn_typed Gamma e%E A%ty) : FType_scope.
+(** Add constructors to [eauto]'s hint database. *)
+#[export] Hint Constructors syn_typed : core.
+Local Open Scope FType_scope.
+(** Also export the notation (it would otherwise remain local to this file). *)
+Notation "Gamma |- e : A" := (syn_typed Gamma e%E A%ty).
+
+(** some small examples *)
+Goal [] |- (lam: 1 + ^0)%E : (Int -> Int).
+Proof. eauto. Qed.
+Goal [Int] |- (lam: ^1 + ^0)%E : (Int -> Int).
+Proof. eauto. Qed.
+Goal [Int; Int -> Int] |- (^1 ^0)%E : Int.
+Proof. eauto. Qed.
+
+(** We derive some inversion lemmas -- this is cleaner than directly
+using the [inversion] tactic everywhere.*)
+Lemma var_inversion Gamma (x : var) A :
+  Gamma |- Var x : A -> Gamma !! x = Some A.
+Proof. inversion 1; subst; auto. Qed.
+
+Lemma lam_inversion Gamma e C :
+  (Gamma |- (lam: e) : C) ->
+  exists A B, C = (A -> B)%ty /\ A :: Gamma |- e : B.
+Proof. inversion 1; subst; eauto. Qed.
+
+Lemma lit_int_inversion Gamma (n : Z) A : (Gamma |- n : A) -> A = Int.
+Proof. inversion 1; subst; auto. Qed.
+
+Lemma app_inversion Gamma e1 e2 B :
+  (Gamma |- e1 e2 : B) ->
+  exists A,  Gamma |- e1 : (A -> B) /\ Gamma |- e2 : A.
+Proof. inversion 1; subst; eauto. Qed.
+
+Lemma plus_inversion Gamma e1 e2 B :
+  (Gamma |- e1 + e2 : B) ->
+  B = Int /\ Gamma |- e1 : Int /\ Gamma |- e2 : Int.
+Proof. inversion 1; subst; eauto. Qed.
+
+(** * Progress *)
+
+(** Canonical forms lemmas *)
+Lemma canonical_values_arr Gamma e A B :
+  Gamma |- e : (A -> B) ->
+  is_val e ->
+  exists e', e = (lam: e')%E.
+Proof.
+  intros He [v ->]. inversion He; destruct v; simplify_eq; by eauto.
+Qed.
+
+Lemma canonical_values_int Gamma e :
+  Gamma |- e : Int ->
+  is_val e ->
+  exists n: Z, e = n.
+Proof.
+  intros He [v ->]. inversion He; destruct v; simplify_eq; by eauto.
+Qed.
+
+Definition progressive (e : expr) :=
+  is_val e \/ exists e', contextual_step e e'.
+
+Theorem type_progress e A :
+  [] |- e : A -> progressive e.
+(* CLASS *) Proof.
+  remember [] as Gamma. induction 1 as [??? Hx| | | Gamma e1 e2 A B Hty IH1 _ IH2 | Gamma e1 e2 Hty1 IH1 Hty2 IH2].
+  - subst. rewrite lookup_nil in Hx. done.
+  - left. by eauto.
+  - left. by eauto.
+  - destruct (IH2 HeqGamma) as [H2|H2]; [destruct (IH1 HeqGamma) as [H1|H1]|].
+    + eapply canonical_values_arr in Hty as (e & ->); last done.
+      right. eexists.
+      eapply base_contextual_step, BetaS; eauto.
+    + right. destruct H2 as [v ->].
+      destruct H1 as [e1' Hstep].
+      eexists. eapply (fill_contextual_step [AppLCtx v]). done.
+    + right. destruct H2 as [e2' H2].
+      eexists. eapply (fill_contextual_step [AppRCtx e1]). done.
+  - destruct (IH2 HeqGamma) as [H2|H2]; first destruct (IH1 HeqGamma) as [H1|H1].
+    + right. eapply canonical_values_int in Hty1 as [n1 ->]; last done.
+      eapply canonical_values_int in Hty2 as [n2 ->]; last done.
+      eexists. eapply base_contextual_step. eapply PlusS; eauto.
+    + right. destruct H2 as [v ->].
+      destruct H1 as [e1' Hstep].
+      eexists. eapply (fill_contextual_step [PlusLCtx v]). done.
+    + right. destruct H2 as [e2' H2].
+      eexists. eapply (fill_contextual_step [PlusRCtx e1]). done.
+Qed.
+
+(** * Preservation *)
+
+(** Helper lemmas for base preservation *)
+
+(** The weakening and substitution lemmas change significantly with De Bruijn
+indices. First we have to generalize our idea of "weakening" to renamings that
+preserve typing from one context to another. Basically, [sigma] tells us "how"
+[Gamma] is included in [Delta] by showing, for each type in [Gamma], where we can find
+the same type in [Delta]. *)
+Definition typed_ren (Gamma Delta : typing_context) (delta : var -> var) :=
+  forall x B, Gamma !! x = Some B -> Delta !! (delta x) = Some B.
+
+(** [ctx_incl] is preserved when both context get identically extended with
+a new type at position 0, and [sigma] is shifted up by 1. *)
+Lemma typed_ren_cons delta Gamma Delta A :
+  typed_ren Gamma Delta delta ->
+  typed_ren (A :: Gamma) (A :: Delta) (upren delta).
+Proof.
+  intros Hdelta [|x] C; simpl; eauto.
+Qed.
+
+(** Lemma 26 *)
+Lemma type_renaming e Gamma (delta : var -> var) Delta A :
+  typed_ren Gamma Delta delta ->
+  Gamma |- e : A ->
+  Delta |- e.[ren delta] : A.
+Proof.
+  intros Hdelta. induction 1 in Delta, delta, Hdelta.
+  (* The [asimpl] tactic understands the properties of substituions and uses them
+  to simplify the goal. *)
+  all: asimpl.
+  - constructor. eapply Hdelta. done.
+  - constructor. eapply IHsyn_typed. eapply typed_ren_cons. done.
+  - eauto.
+  - eauto.
+  - eauto.
+Qed.
+
+(** For the substitution lemma, we introduce the idea of a type-preserving
+substitution. Note that this is very similar to [ctx_incl], but instead of
+[Delta !! (delta x) = Some B] (which only makes sense when [delta x] is a
+variable) we know have [Delta |- sigma x : B] (which makes sense even when
+[sigma x] is an arbitrary term). *)
+Definition typed_subst (Gamma Delta : typing_context) (sigma : var -> expr) :=
+  forall x B, Gamma !! x = Some B -> Delta |- sigma x : B.
+
+(** On renamings, [typed_ren] and [typed_subst] are equivalent. *)
+Lemma typed_subst_ren (Gamma Delta : typing_context) (delta : var -> var) :
+  typed_ren Gamma Delta delta <-> typed_subst Gamma Delta (ren delta).
+Proof.
+  split.
+  - intros Hdelta x B Hx. specialize (Hdelta _ _ Hx). by constructor.
+  - intros Hdelta x B Hx. specialize (Hdelta _ _ Hx). by inversion Hdelta.
+Qed.
+
+(** [subst_typed] is preserved when both context get identically extended with
+a new type at position 0, and [sigma] is shifted up by 1. *)
+Lemma typed_subst_cons sigma Gamma Delta A :
+  typed_subst Gamma Delta sigma ->
+  typed_subst (A :: Gamma) (A :: Delta) (up sigma).
+Proof.
+  intros Hsigma [|x] B; asimpl.
+  + intros [= ->]. eauto.
+  + intros Hx. specialize (Hsigma _ _ Hx).
+    eapply type_renaming; last done.
+    intros y B'. asimpl. eauto.
+Qed.
+
+(** The substitution [e .: ids] corresponds to what happens when substitution
+with [e/]: it replaces variable 0 with [e] and shifts everything down by one.
+This lemma shows the type of that substitution. *)
+Lemma typed_subst_cons_l Gamma A e :
+  Gamma |- e : A ->
+  typed_subst (A::Gamma) Gamma (e .: ids).
+Proof.
+  intros He [|x] C; simpl; intros Hx.
+  - simplify_eq. done.
+  - eauto.
+Qed.
+
+(** Lemma 27 *)
+Lemma type_substitution e Gamma sigma Delta A :
+  typed_subst Gamma Delta sigma ->
+  Gamma |- e : A ->
+  Delta |- e.[sigma] : A.
+Proof.
+  intros Hsigma. induction e in Gamma, A, Delta, sigma, Hsigma |- *.
+  - intros Hp%var_inversion. asimpl. eapply Hsigma. done.
+  - intros (C & D & -> & Hty)%lam_inversion. asimpl.
+    econstructor. eapply IHe; last done. by eapply typed_subst_cons.
+  - intros (C & Hty1 & Hty2)%app_inversion. asimpl. eauto.
+  - intros ->%lit_int_inversion. asimpl. eauto.
+  - intros (-> & Hty1 & Hty2)%plus_inversion. asimpl. eauto.
+Qed.
+
+(** Lemma 28: We can derive a substitution lemma for single-variable substitution.
+Note how this is significantly stronger than the version we proved for string-based
+substitution! [e'] can now use the variables in [Gamma], which the previous
+lemma did not allow. This is because previously we needed [e'] to be a closed
+term to avoid the problems with capturing substitution, but now with De Bruijn
+indices we have a proper capture-avoiding substitution. *)
+Lemma type_substitution_one e e' Gamma A B :
+  Gamma |- e' : B ->
+  B :: Gamma |- e : A ->
+  Gamma |- e.[e'/] : A.
+Proof.
+  intros. eapply type_substitution; last done.
+  eapply typed_subst_cons_l. done.
+Qed.
+
+(** Base preservation *)
+Lemma type_preservation_base_step e e' A :
+  [] |- e : A ->
+  base_step e e' ->
+  [] |- e' : A.
+Proof.
+  intros Hty Hstep. destruct Hstep as [| e1 e2 n1 n2 n3 Heq1 Heq2 Heval]; subst.
+  - eapply app_inversion in Hty as (B & Hty1 & Hty2).
+    eapply lam_inversion in Hty1 as (B' & A' & Heq1 & Hty).
+    simplify_eq. eapply type_substitution_one; done.
+  - eapply plus_inversion in Hty as (-> & Hty1 & Hty2).
+    econstructor.
+Qed.
+
+(** Contextual typing for evaluation context items and evaluation contexts  *)
+Definition ectx_item_typing (Ki : ectx_item) (A B : type) :=
+  forall e, [] |- e : A -> [] |- (fill_item Ki e) : B.
+
+Lemma fill_item_typing_decompose Ki e A :
+  [] |- fill_item Ki e : A ->
+  exists B, [] |- e : B /\ ectx_item_typing Ki B A.
+(* CLASS *) Proof.
+  unfold ectx_item_typing; destruct Ki; simpl; inversion 1; subst; eauto.
+Qed.
+
+Definition ectx_typing (K : ectx) (A B : type) :=
+  forall e, [] |- e : A -> [] |- (fill K e) : B.
+
+Lemma fill_typing_decompose K e A :
+  [] |- fill K e : A ->
+  exists B, [] |- e : B /\ ectx_typing K B A.
+(* CLASS *) Proof.
+  unfold ectx_typing. induction K as [|k K] in e |- *; simpl; eauto.
+  intros [B [Hit Hty]]%IHK.
+  eapply fill_item_typing_decompose in Hit as [B' [? ?]]; eauto.
+Qed.
+
+Lemma fill_typing_compose K e A B :
+  [] |- e : B ->
+  ectx_typing K B A ->
+  [] |- fill K e : A.
+(* CLASS *) Proof.
+  intros H1 H2; by eapply H2.
+Qed.
+
+(** Preservation *)
+Theorem type_preservation e e' A :
+  [] |- e : A ->
+  contextual_step e e' ->
+  [] |- e' : A.
+(* CLASS *) Proof.
+  intros Hty Hstep. destruct Hstep as [K e1 e2 -> -> Hstep].
+  eapply fill_typing_decompose in Hty as [B [H1 H2]].
+  eapply fill_typing_compose; last done.
+  by eapply type_preservation_base_step.
+Qed.
+
+(** And finally: Type Safety *)
+Corollary type_safety e1 e2 A:
+  [] |- e1 : A ->
+  rtc contextual_step e1 e2 ->
+  progressive e2.
+(* REMOVE *) Proof.
+  induction 2; eauto using type_progress, type_preservation.
+Qed.
